LeanColls/Array/VarArray.lean
@@ -1,0 +1,21 @@
+/-
+Copyright (c) 2022 James Gallicchio.
+
+Authors: James Gallicchio
+-/
+
+import LeanColls.Array.COWArray
+
+namespace LeanColls
+
+structure VarArray (α) where
+  size : Nat
+  backing : COWArray α size
+
+namespace VarArray
+
+instance : Indexed (VarArray α) α where
+  size a := a.size
+  nth a i := a.backing.get i
+
+def empty : VarArray α := ⟨0, COWArray.empty⟩
